\setcounter{section}{4}
\section{Challenge Activity 5 - Regular Expressions}
{
\renewcommand{\thesubsection}{\thesection.\alph{subsection}}
\subsection{Item a}
\begin{theorem}
If $L((01+10)(01+10)^\ast)$, then
\begin{equation*}
	\forall w \in L, \#0(w)=\#1(w)
\end{equation*}
\end{theorem}
\begin{proof}
Base case: $w=01$. The theorem applies trivially given that $\#0(w)=\#1(w) \iff 1=1$.\\
Base case: $w=10$. The theorem applies trivially given that $\#0(w)=\#1(w) \iff 1=1$.\\
Inductive hypothesis: $\#0(w)=\#1(w)$\\
Inductive step: $w'=w01$
\begin{alignat*}{2}
	\#0(w')=\#1(w')
	&\iff \#0(w01)      &&=\#1(w01)\\
	&\iff \#0(w)+\#0(01)&&=\#1(w)+\#1(01)\\
	&\iff \#0(w)+1      &&=\#1(w)+1\\
	&\iff \#0(w)        &&=\#1(w)
\end{alignat*}
Inductive step: $w'=w10$
\begin{alignat*}{2}
	\#0(w')=\#1(w')
	&\iff \#0(w10)      &&=\#1(w10)\\
	&\iff \#0(w)+\#0(10)&&=\#1(w)+\#1(10)\\
	&\iff \#0(w)+1      &&=\#1(w)+1\\
	&\iff \#0(w)        &&=\#1(w)
\end{alignat*}
Having proven the theorem holds for the two base cases, and the two inductive steps, we have proven the theorem.
\end{proof}
\subsection{Item b}
\begin{theorem}
	$L=\{w\in \{0,1\}^\ast \colon \#0(w)=\#1(w)\}$ is not a regular language.
\end{theorem}
\begin{proof}
Assume by absurd that
\begin{equation}\label{eq:CA05_ABSURD}
L \text{ is a regular language}
\end{equation}
Then there is a DFA with $N$ states that is equivalent to $L$, where each state represents a distinct value of the difference between \#0 and \#1 up to a certain symbol in a string.\\
Consider $w=0^{N+1}1^{N+1}$. This string would require $N+1$ states to represent the differences between \#0 and \#1 (which would range from $0$ to $N+1$), and thus is not accepted by the DFA. However, $w$ trivially belongs to $L$, thus arriving at a contradiction with \eqref{eq:CA05_ABSURD}.\\
We have thus proven the theorem correct.
\end{proof}
}