\documentclass[docid=PA01]{tcom_PA}
\begin{document}
\setcounter{chapter}{0}
\exam{Preparation Activity 1 - Proof by Induction}
\begin{theorem}
	\begin{equation*}
		\forall x \in \mathbb{R}\setminus \{0,1\},\forall n \in \mathbb{N}, \sum_{i=0}^{n}{x^i} = \frac{x^{n+1}-1}{x-1}
	\end{equation*}
\end{theorem}
\begin{proof}
Base case: $n=0$
\begin{alignat*}{2}
	\sum_{i=0}^{n}{x^i} = \frac{x^{n+1}-1}{x-1}
	&\iff \sum_{i=0}^{0}{x^i} &&= \frac{x^{0+1}-1}{x-1}\\
	&\iff x^0                 &&= \frac{x-1}{x-1}
\end{alignat*}
Given $x \neq 0$ and $x \neq 1$, the above equation is trivially true.\\
Inductive hypothesis:
\begin{equation*}
\sum_{i=0}^{n}{x^i} = \frac{x^{n+1}-1}{x-1}
\end{equation*}
Inductive step:
\begin{alignat*}{3}
	\sum_{i=0}^{n+1}{x^i} = \frac{x^{n+2}-1}{x-1}
	&\iff x^{n+1}         &&+\sum_{i=0}^{n}{x^i}   &&= \frac{x^{n+2}-1}{x-1}\\
	&\iff x^{n+1}         &&+\frac{x^{n+1}-1}{x-1} &&= \frac{x^{n+2}-1}{x-1}\\
	&\iff (x-1)x^{n+1}    &&+x^{n+1}-1             &&= x^{n+2}-1\\
	&\iff x^{n+2}-x^{n+1} &&+x^{n+1}               &&= x^{n+2}\\
\end{alignat*}
Having proven the theorem correct for the base case and the inductive step, the theorem is proven.
\end{proof}
\end{document}
